proof/agp32CorrectScript.sml
@@ -1,4 +1,4 @@
-open hardwarePreamble translatorTheory translatorLib arithmeticTheory dep_rewrite blastLib bitstringSyntax fcpSyntax listSyntax wordsSyntax agp32StateTheory agp32EnvironmentTheory agp32ProcessorTheory ag32Theory ag32ExtraTheory ag32UtilitiesTheory agp32RelationTheory agp32UpdateTheory agp32InternalTheory agp32StepLib agp32_IF_CorrectTheory agp32_ID_CorrectTheory;
+open hardwarePreamble translatorTheory translatorLib arithmeticTheory dep_rewrite blastLib bitstringSyntax fcpSyntax listSyntax wordsSyntax agp32StateTheory agp32EnvironmentTheory agp32ProcessorTheory ag32Theory ag32ExtraTheory ag32UtilitiesTheory agp32RelationTheory agp32UpdateTheory agp32InternalTheory agp32StepLib agp32_IF_CorrectTheory agp32_ID_CorrectTheory agp32_EX_CorrectTheory;
 
 (* correctness of the pipelined Silver circuit against the ISA *)
 val _ = new_theory "agp32Correct";
@@ -6,302 +6,16 @@ val _ = new_theory "agp32Correct";
 val _ = prefer_num ();
 val _ = guess_lengths ();
 
-(* MARK: keep it here for EX proof later
-(* tactic *)
-val update_carry_flag_when_enabled_tac =
-    (Q.ABBREV_TAC `s = agp32 fext fbits t` >>
-     Q.ABBREV_TAC `s' = procs [agp32_next_state;WB_pipeline;MEM_pipeline;EX_pipeline;
-                               REG_write;ID_pipeline;IF_PC_update;Acc_compute]
-                              (fext t) s s` >>
-     Q.ABBREV_TAC `s'' = procs [ForwardA;ForwardB;ForwardW;IF_instr_update;
-                                ID_opc_func_update;ID_imm_update;
-                                ID_data_update;EX_ctrl_update;EX_forward_data;
-                                EX_ALU_input_update;EX_compute_enable_update]
-                               (fext (SUC t)) s' s'` >>                        
-     `(agp32 fext fbits (SUC t)).EX.EX_carry_flag =
-     (EX_ALU_update (fext (SUC t)) s' s'').EX.EX_carry_flag`
-       by fs [agp32_EX_ALU_items_updated_by_EX_ALU_update,Abbr `s`,Abbr `s'`,Abbr `s''`] >> rw []);
 
-val carry_flag_unchanged_tac =
-    (Q.ABBREV_TAC `s3 = procs [agp32_next_state;WB_pipeline;MEM_pipeline] (fext t) s s` >>
-     `?s4.(agp32 fext fbits (SUC t)).EX.EX_opc = (EX_pipeline (fext (SUC t)) s4 s3).EX.EX_opc`
-       by fs [agp32_EX_opc_func_updated_by_EX_pipeline,Abbr `s3`,Abbr `s`] >>
-     `(s3.ID.ID_EX_write_enable <=> s.ID.ID_EX_write_enable) /\ (s3.ID.ID_opc = s.ID.ID_opc)`
-       by METIS_TAC [Abbr `s3`,Abbr `s`,agp32_same_items_until_MEM_pipeline] >>
-     `s3.ID.ID_EX_write_enable` by fs [enable_stg_def] >>
-      Cases_on `enable_stg 2 s` >-
-      ((** ID is enabled at cycle t **)
-       `s.ID.ID_opc = opc ai` by (fs [Rel_def] >> `2 = 3 - 1 /\ 3 <> 1` by rw [] >>
-                              `I' (3,SUC t) = I' (2,t)` by METIS_TAC [Abbr `s`] >>
-                              fs [ID_Rel_def]) >>
-       `((agp32 fext fbits (SUC t)).EX.EX_opc = 16w) \/
-       ((agp32 fext fbits (SUC t)).EX.EX_opc = s.ID.ID_opc)`
-         by (fs [EX_pipeline_def] >> Cases_on `s3.EX.EX_NOP_flag` >> fs []) >>
-       `(s''.EX.EX_opc = (agp32 fext fbits (SUC t)).EX.EX_opc) /\
-       (s''.EX.EX_func = (agp32 fext fbits (SUC t)).EX.EX_func)`
-         by METIS_TAC [agp32_same_EX_opc_func_until_ALU_update,Abbr `s`,Abbr `s'`,Abbr `s''`] >>
-       `(s''.EX.EX_func = 9w) \/ (s''.EX.EX_func = 12w) \/ (s''.EX.EX_func = 13w) \/
-       (s''.EX.EX_func = 14w) \/ (s''.EX.EX_func = 15w)`
-         by fs [Abbr `s`,agp32_EX_opc_implies_EX_func] >>
-       `s''.EX.EX_carry_flag <=> s.EX.EX_carry_flag`
-         by METIS_TAC [agp32_same_EX_carry_flag_as_before,Abbr `s`,Abbr `s'`,Abbr `s''`] >>
-       rw [EX_ALU_update_def] >> fs [Rel_def,Abbr `s`]) >>
-     (** ID is disabled at cycle t **)
-     `s.EX.EX_NOP_flag` by fs [Abbr `s`,agp32_ID_enable_flags_imply_flush_NOP_flags,enable_stg_def] >>
-     `s3.EX.EX_NOP_flag <=> s.EX.EX_NOP_flag` by METIS_TAC [Abbr `s3`,Abbr `s`,agp32_same_items_until_MEM_pipeline] >>
-     fs [EX_pipeline_def] >>
-     `(s''.EX.EX_opc = (agp32 fext fbits (SUC t)).EX.EX_opc) /\
-     (s''.EX.EX_func = (agp32 fext fbits (SUC t)).EX.EX_func)`
-       by METIS_TAC [agp32_same_EX_opc_func_until_ALU_update,Abbr `s`,Abbr `s'`,Abbr `s''`] >>
-     `(s''.EX.EX_func = 9w) \/ (s''.EX.EX_func = 12w) \/ (s''.EX.EX_func = 13w) \/
-     (s''.EX.EX_func = 14w) \/ (s''.EX.EX_func = 15w)`
-       by fs [Abbr `s`,agp32_EX_opc_implies_EX_func] >>
-     `s''.EX.EX_carry_flag <=> s.EX.EX_carry_flag`
-       by METIS_TAC [agp32_same_EX_carry_flag_as_before,Abbr `s`,Abbr `s'`,Abbr `s''`] >>    
-     rw [EX_ALU_update_def] >> fs [Rel_def,Abbr `s`]);
-
-val carry_flag_unchanged_by_func_tac =
-    (Q.ABBREV_TAC `s3 = procs [agp32_next_state;WB_pipeline;MEM_pipeline] (fext t) s s` >>
-     `?s4.(agp32 fext fbits (SUC t)).EX.EX_func = (EX_pipeline (fext (SUC t)) s4 s3).EX.EX_func`
-       by fs [agp32_EX_opc_func_updated_by_EX_pipeline,Abbr `s3`,Abbr `s`] >>
-     `(s3.ID.ID_EX_write_enable <=> s.ID.ID_EX_write_enable) /\ (s3.ID.ID_func = s.ID.ID_func)`
-       by METIS_TAC [Abbr `s3`,Abbr `s`,agp32_same_items_until_MEM_pipeline] >>
-     `s3.ID.ID_EX_write_enable` by fs [enable_stg_def] >>
-      Cases_on `enable_stg 2 s` >-
-      ((** ID is enabled at cycle t **)
-       `s.ID.ID_func = func ai` by (fs [Rel_def] >> `2 = 3 - 1 /\ 3 <> 1` by rw [] >>
-                                    `I' (3,SUC t) = I' (2,t)` by METIS_TAC [Abbr `s`] >>
-                                    fs [ID_Rel_def]) >>
-       `((agp32 fext fbits (SUC t)).EX.EX_func = 12w) \/
-       ((agp32 fext fbits (SUC t)).EX.EX_func = s.ID.ID_func)`
-         by (fs [EX_pipeline_def] >> Cases_on `s3.EX.EX_NOP_flag` >> fs []) >>
-       `s''.EX.EX_func = (agp32 fext fbits (SUC t)).EX.EX_func`
-         by METIS_TAC [agp32_same_EX_opc_func_until_ALU_update,Abbr `s`,Abbr `s'`,Abbr `s''`] >>
-       `(s''.EX.EX_func <> 0w) /\ (s''.EX.EX_func <> 1w)` by fs [] >>
-       `s''.EX.EX_carry_flag <=> s.EX.EX_carry_flag`
-         by METIS_TAC [agp32_same_EX_carry_flag_as_before,Abbr `s`,Abbr `s'`,Abbr `s''`] >>
-       rw [EX_ALU_update_def] >> fs [Rel_def,Abbr `s`] >>
-       Cases_on_word_value `func ai` >> fs []) >>
-     (** ID is disabled at cycle t **)
-     `s.EX.EX_NOP_flag` by fs [Abbr `s`,agp32_ID_enable_flags_imply_flush_NOP_flags,enable_stg_def] >>
-     `s3.EX.EX_NOP_flag <=> s.EX.EX_NOP_flag` by METIS_TAC [Abbr `s3`,Abbr `s`,agp32_same_items_until_MEM_pipeline] >>
-     fs [EX_pipeline_def] >>
-     `s''.EX.EX_func = (agp32 fext fbits (SUC t)).EX.EX_func`
-       by METIS_TAC [agp32_same_EX_opc_func_until_ALU_update,Abbr `s`,Abbr `s'`,Abbr `s''`] >>
-     `s''.EX.EX_carry_flag <=> s.EX.EX_carry_flag`
-       by METIS_TAC [agp32_same_EX_carry_flag_as_before,Abbr `s`,Abbr `s'`,Abbr `s''`] >>    
-     rw [EX_ALU_update_def] >> fs [Rel_def,Abbr `s`]);
-
-(* lemmas *)
-(** lemmas copied from the hardware/ag32 repo **)
-Theorem ALU_correct_carry_lem:
-  !(w:33 word). word_bit 32 w <=> n2w (dimword(:32)) <=+ w
+(* lemma *)
+Theorem agp32_data_in_unchanged_all:
+  !fext t.
+    is_data_in fext ==>
+    (fext t).data_in = (fext 0).data_in
 Proof
-  simp [] >> BBLAST_PROVE_TAC
+  rw [is_data_in_def] >>
+  Induct_on `t` >> fs []
 QED
-
-Theorem ALU_correct_v2w_carry33_lem:
-  !b. v2w [b] = if b then (1w:33 word) else 0w
-Proof
-  Cases >> EVAL_TAC
-QED
-(** copy end **)
-                                              
-Theorem w2n_add_MOD_itself:
-  !(w1:word32) (w2:word32).
-    w2n w1 + w2n w2 = (w2n w1 + w2n w2) MOD 8589934592
-Proof
-  rw [] >>
-  `(w2n w1 < 4294967296) /\ (w2n w2 < 4294967296)` by METIS_TAC [w2n_lt,dimword_32] >>
-  fs []
-QED
-
-(* carry_flag between ISA and circuit states *)
-Theorem agp32_Rel_ag32_carry_flag_correct:
-  !fext fbits a t I.
-    (!t k. enable_stg k (agp32 fext fbits t) ==> k <> 1 ==>
-           (I (k,SUC t) = I (k,t) + 1) /\ (I (k,SUC t) = I (k - 1,t))) ==>
-    (!t k. ~enable_stg k (agp32 fext fbits t) ==> I (k,SUC t) = I (k,t)) ==>
-    Rel I (fext t) (agp32 fext fbits (t-1)) (agp32 fext fbits t) a t ==>
-    ((agp32 fext fbits (SUC t)).EX.EX_carry_flag <=>
-     (FUNPOW Next (I (3,SUC t)) a).CarryFlag)
-Proof
-  rw [] >> Cases_on `enable_stg 3 (agp32 fext fbits t)` >-
-   (** EX stage is enabled **)
-   (`I'(3,SUC t) = SUC (I'(3,t))` by fs [] >>
-    rw [FUNPOW_SUC] >>
-    Q.ABBREV_TAC `ai = FUNPOW Next (I' (3,t)) a` >>             
-    rw [Next_def,GSYM word_at_addr_def,GSYM align_addr_def] >>
-    Cases_on `Decode (word_at_addr ai.MEM (align_addr ai.PC))` >-
-
-     ((** Accelerator **)
-     PairCases_on `p` >> rw [Run_def,dfn'Accelerator_def,incPC_def] >>
-     update_carry_flag_when_enabled_tac >>
-     `opc ai = 8w` by fs [ag32_Decode_Acc_opc_8w] >>
-     carry_flag_unchanged_tac) >-   
-
-     ((** In **)
-     rw [Run_def,dfn'In_def,incPC_def] >>
-     update_carry_flag_when_enabled_tac >>
-     `opc ai = 7w` by fs [ag32_Decode_In_opc_7w] >>
-     carry_flag_unchanged_tac) >-
-
-     ((** Interrupt **)
-     rw [Run_def,dfn'Interrupt_def,incPC_def] >>
-     update_carry_flag_when_enabled_tac >>
-     `opc ai = 12w` by fs [ag32_Decode_Interrupt_opc_12w] >>
-     carry_flag_unchanged_tac) >-
-
-     ((** Jump: CarryFlag can be changed **)
-     PairCases_on `p` >> rw [Run_def,dfn'Jump_def] >>
-     pairarg_tac >> fs [] >>
-     Cases_on `p0 = fAdd` >-
-      ((** fAdd **)
-      fs [ALU_def] >> rw [] >>
-      update_carry_flag_when_enabled_tac >>
-      `func ai = 0w` by fs [ag32_Decode_Jump_fAdd_func_0w] >>
-      `s''.EX.EX_func = 0w` by cheat >>
-      `s''.EX.EX_compute_enable` by cheat >>
-      rw [EX_ALU_update_def,ALU_correct_carry_lem,WORD_LS,word_add_def,w2n_w2w] >>
-      `(s''.EX.EX_ALU_input1 = ai.PC) /\ (s''.EX.EX_ALU_input2 = ri2word p2 ai)` by cheat >>
-      rw [] >> METIS_TAC [w2n_add_MOD_itself]) >>
-     Cases_on `p0 = fAddWithCarry` >-
-      ((** fAddWithCarry **)
-      fs [ALU_def] >> rw [] >>
-      cheat) >>
-     `s.CarryFlag = ai.CarryFlag` by (fs [ALU_def] >> Cases_on `p0` >> fs [] >> rw []) >>
-     fs [] >> rename1 `(v,ai')` >>
-     update_carry_flag_when_enabled_tac >>
-     `(func ai <> 0w) /\ (func ai <> 1w)` by fs [ag32_Decode_Jump_func_not_0w_1w] >>
-     carry_flag_unchanged_by_func_tac) >-
-
-     ((** JumpIfNotZero: CarryFlag can be changed **)
-     PairCases_on `p` >> rw [Run_def,dfn'JumpIfNotZero_def] >>
-     pairarg_tac >> fs [] >>
-     Cases_on `p0 = fAdd` >-
-      ((** fAdd **)
-      fs [ALU_def,incPC_def] >> rw [] >>
-      cheat) >>
-     Cases_on `p0 = fAddWithCarry` >-
-      ((** fAddWithCarry **)
-      fs [ALU_def,incPC_def] >> rw [] >>
-      cheat) >>
-     `s.CarryFlag = ai.CarryFlag` by (fs [ALU_def] >> Cases_on `p0` >> fs [] >> rw []) >>
-     fs [] >> rename1 `(v,ai')` >>
-     update_carry_flag_when_enabled_tac >> rw [incPC_def] >>
-     `(func ai <> 0w) /\ (func ai <> 1w)` by fs [ag32_Decode_JumpIfNotZero_func_not_0w_1w] >>
-     carry_flag_unchanged_by_func_tac) >-
-
-     ((** JumpIfZreo: CarryFlag can be changed **)
-     PairCases_on `p` >> rw [Run_def,dfn'JumpIfZero_def] >>
-     pairarg_tac >> fs [] >>
-     Cases_on `p0 = fAdd` >-
-      ((** fAdd **)
-      fs [ALU_def,incPC_def] >> rw [] >>
-      cheat) >>
-     Cases_on `p0 = fAddWithCarry` >-
-      ((** fAddWithCarry **)
-      fs [ALU_def,incPC_def] >> rw [] >>
-      cheat) >>
-     `s.CarryFlag = ai.CarryFlag` by (fs [ALU_def] >> Cases_on `p0` >> fs [] >> rw []) >>
-     fs [] >> rename1 `(v,ai')` >>
-     update_carry_flag_when_enabled_tac >> rw [incPC_def] >>
-     `(func ai <> 0w) /\ (func ai <> 1w)` by fs [ag32_Decode_JumpIfZero_func_not_0w_1w] >>
-     carry_flag_unchanged_by_func_tac) >-
-
-     ((** LoadConstant **)
-     PairCases_on `p` >> rw [Run_def,dfn'LoadConstant_def,incPC_def] >>
-     update_carry_flag_when_enabled_tac >>
-     `opc ai = 13w` by fs [ag32_Decode_LoadConstant_opc_13w] >>
-     carry_flag_unchanged_tac) >-
-
-     ((** LoadMEM **)
-     PairCases_on `p` >> rw [Run_def,dfn'LoadMEM_def,incPC_def] >>
-     update_carry_flag_when_enabled_tac >>
-     `opc ai = 4w` by fs [ag32_Decode_LoadMEM_opc_4w] >>
-     carry_flag_unchanged_tac) >-
-
-     ((** LoadMEMByte **)
-     PairCases_on `p` >> rw [Run_def,dfn'LoadMEMByte_def,incPC_def] >>
-     update_carry_flag_when_enabled_tac >>
-     `opc ai = 5w` by fs [ag32_Decode_LoadMEMByte_opc_5w] >>
-     carry_flag_unchanged_tac) >-
-
-     ((** LoadUpperConstant **)
-     PairCases_on `p` >> rw [Run_def,dfn'LoadUpperConstant_def,incPC_def] >>
-     update_carry_flag_when_enabled_tac >>
-     `opc ai = 14w` by fs [ag32_Decode_LoadUpperConstant_opc_14w] >>
-     carry_flag_unchanged_tac) >-
-
-     ((** Normal: CarryFlag can be changed **)
-     PairCases_on `p` >> rw [Run_def,dfn'Normal_def,norm_def,incPC_def] >>
-     pairarg_tac >> fs [] >>
-     Cases_on `p0 = fAdd` >-
-      ((** fAdd **)
-      fs [ALU_def] >> rw [] >>
-      cheat) >>
-     Cases_on `p0 = fAddWithCarry` >-         
-      ((** fAddWithCarry **)
-      fs [ALU_def] >> rw [] >>
-      cheat) >>
-     `s.CarryFlag = ai.CarryFlag` by (fs [ALU_def] >> Cases_on `p0` >> fs [] >> rw []) >>
-     fs [] >> rename1 `(v,ai')` >>
-     update_carry_flag_when_enabled_tac >>
-     `(func ai <> 0w) /\ (func ai <> 1w)` by fs [ag32_Decode_Normal_func_not_0w_1w] >>
-     carry_flag_unchanged_by_func_tac) >-
-
-     ((** Out: CarryFlag can be changed **)
-     PairCases_on `p` >> rw [Run_def,dfn'Out_def,norm_def,incPC_def] >>
-     pairarg_tac >> fs [] >>
-     Cases_on `p0 = fAdd` >-
-      ((** fAdd **)
-      fs [ALU_def] >> rw [] >>
-      cheat) >>
-     Cases_on `p0 = fAddWithCarry` >-         
-      ((** fAddWithCarry **)
-      fs [ALU_def] >> rw [] >>
-      cheat) >>
-     `s.CarryFlag = ai.CarryFlag` by (fs [ALU_def] >> Cases_on `p0` >> fs [] >> rw []) >>
-     fs [] >> rename1 `(v,ai')` >>
-     update_carry_flag_when_enabled_tac >>
-     `(func ai <> 0w) /\ (func ai <> 1w)` by fs [ag32_Decode_Out_func_not_0w_1w] >>
-     carry_flag_unchanged_by_func_tac) >-
-
-     ((** ReservedInstr **)
-     rw [Run_def] >>
-     update_carry_flag_when_enabled_tac >>
-     `opc ai = 15w` by fs [ag32_Decode_ReservedInstr_opc_15w] >>
-     carry_flag_unchanged_tac) >-
-
-     ((** Shift **)
-     PairCases_on `p` >> rw [Run_def,dfn'Shift_def,incPC_def] >>
-     update_carry_flag_when_enabled_tac >>
-     `opc ai = 1w` by fs [ag32_Decode_Shift_opc_1w] >>
-     carry_flag_unchanged_tac) >-
-
-     ((** StoreMEM **)
-     PairCases_on `p` >> rw [Run_def,dfn'StoreMEM_def,incPC_def] >>
-     update_carry_flag_when_enabled_tac >>
-     `opc ai = 2w` by fs [ag32_Decode_StoreMEM_opc_2w] >>
-     carry_flag_unchanged_tac) >>
-
-    (** StoreMEMByte **)
-    PairCases_on `p` >> rw [Run_def,dfn'StoreMEMByte_def,incPC_def] >>
-    update_carry_flag_when_enabled_tac >>
-    `opc ai = 3w` by fs [ag32_Decode_StoreMEMByte_opc_3w] >>
-    carry_flag_unchanged_tac) >>
-
-  (** EX stage is disabled **)
-  `I' (3,SUC t) = I' (3,t)` by fs [] >>
-  fs [Rel_def] >>
-  update_carry_flag_when_enabled_tac >>
-  reverse (Cases_on `s''.EX.EX_compute_enable`) >-
-   (`s''.EX.EX_carry_flag <=> s.EX.EX_carry_flag`
-      by METIS_TAC [agp32_same_EX_carry_flag_as_before,Abbr `s`,Abbr `s'`,Abbr `s''`] >>
-    fs [EX_ALU_update_def]) >>
-  cheat
-QED
-*)
 
 
 (* Init relation implies Rel at cycle 0 *)
@@ -312,17 +26,8 @@ Theorem agp32_Init_implies_Rel:
     Init (fext 0) (s 0) a ==>
     Rel I (fext 0) (s 0) (s 0) a 0
 Proof
-  rw [Init_def,Rel_def,is_sch_init_def] >-
-   (* THE NONE problem *)
-   cheat >-
-   cheat >-
-   cheat >-
-   fs [agp32_init_IF_PC_input] >-
-   (* THE NONE problem *)
-   cheat >-
-   cheat >-
-   cheat >>
-  fs [IF_PC_Rel_def,IF_instr_Rel_def,enable_stg_def,reg_data_vaild_def] >> fs []
+  rw [Init_def,Rel_def,is_sch_init_def] >>
+  fs [agp32_init_IF_PC_input,IF_PC_Rel_def,IF_instr_Rel_def,enable_stg_def,reg_data_vaild_def] >> fs []
 QED
 
 
@@ -345,7 +50,9 @@ Proof
   `Rel I' (fext t) (s (t-1)) (s t) a t` by METIS_TAC [] >>
   rw [Rel_def] >-
    (** data_in **)
-   fs [Rel_def,is_data_in_def,ag32_data_in_unchanged_all] >-
+   (fs [agp32_data_in_unchanged_all,Init_def] >>
+    `a.data_in = (FUNPOW Next 0 a).data_in` by rw [] >>
+    METIS_TAC [ag32_data_in_unchanged_all]) >-
    (** carryflag **)
    (*METIS_TAC [agp32_Rel_ag32_carry_flag_correct]*)
    cheat >-
@@ -371,12 +78,14 @@ Proof
    fs [agp32_Rel_ag32_IF_instr_Rel_correct] >-
    (** ID **)
    fs [is_sch_def,agp32_Rel_ag32_ID_Rel_correct] >-
-   (** EX **)
+   (** EX_Rel **)
+   fs [is_sch_def,agp32_Rel_ag32_EX_Rel_correct] >-
+   (** EX_Rel_spec **)
    cheat >-
    (** MEM **)
    cheat >>
-   (** WB **)
-   cheat
+  (** WB **)
+  cheat
 QED
 
 val _ = export_theory ();
